Logic/Propositional/Structural/Classical.lean
@@ -1,0 +1,124 @@
+namespace Logic.Propositional.Structural.Classical
+
+opaque BasePropn : Type
+
+inductive Propn
+  | base (P : BasePropn)
+  | true
+  | false
+  | not (A : Propn)
+  | and (A B : Propn)
+  | or (A B : Propn)
+
+inductive Ctx
+  | nil
+  | cons (Γ : Ctx) (A : Propn)
+
+inductive Mem (A : Propn) : (Γ : Ctx) → Type
+  | here : Mem A (.cons Γ A)
+  | there (u : Mem A Γ) : Mem A (Γ.cons B)
+
+def Rename (Γ Γ' : Ctx) : Type :=
+  ∀ ⦃A⦄, (u : Mem A Γ) → Mem A Γ'
+
+def Rename.id : Rename Γ Γ
+  | _, u => u
+
+def Rename.weakening : Rename Γ (Γ.cons A)
+  | _ => .there
+
+def Rename.contraction (u : Mem A Γ) : Rename (Γ.cons A) Γ
+  | _, .here => u
+  | _, .there u => u
+
+def Rename.exchange : Rename (Ctx.cons Γ A |>.cons B) (Γ.cons B |>.cons A)
+  | _, .here => .there .here
+  | _, .there .here => .here
+  | _, .there (.there u) => u.there.there
+
+def Rename.cons (γ : Rename Γ Γ') {A} : Rename (Γ.cons A) (Γ'.cons A)
+  | _, .here => .here
+  | _, .there u => (γ u).there
+
+-- Sequent Calculus
+namespace SC
+
+inductive Seq : (Γ : Ctx) → (Δ : Ctx) → Type
+  | id (u : Mem (.base P) Γ) (v : Mem (.base P) Δ) : Seq Γ Δ
+  | trueR (v : Mem .true Δ) : Seq Γ Δ
+  | falseL (u : Mem .false Γ) : Seq Γ Δ
+  | notR (v : Mem A.not Δ) (D : Seq (Γ.cons A) Δ) : Seq Γ Δ
+  | notL (u : Mem A.not Γ) (D : Seq Γ (Δ.cons A)) : Seq Γ Δ
+  | andR (v : Mem (A.and B) Δ) (D₁ : Seq Γ (Δ.cons A)) (D₂ : Seq Γ (Δ.cons B)) : Seq Γ Δ
+  | andL₁ (u : Mem (A.and B) Γ) (D : Seq (Γ.cons A) Δ) : Seq Γ Δ
+  | andL₂ (u : Mem (.and A B) Γ) (D : Seq (Γ.cons B) Δ) : Seq Γ Δ
+  | orR₁ (v : Mem (A.or B) Δ) (D : Seq Γ (Δ.cons A)) : Seq Γ Δ
+  | orR₂ (v : Mem (.or A B) Δ) (D : Seq Γ (Δ.cons B)) : Seq Γ Δ
+  | orL (u : Mem (A.or B) Γ) (D₁ : Seq (Γ.cons A) Δ) (D₂ : Seq (Γ.cons B) Δ) : Seq Γ Δ
+
+def Seq.rename (γ : Rename Γ Γ') (δ : Rename Δ Δ') : (D : Seq Γ Δ) → Seq Γ' Δ'
+  | id u v => id (γ u) (δ v)
+  | trueR v => trueR (δ v)
+  | falseL u => falseL (γ u)
+  | notR v D => notR (δ v) (D.rename γ.cons δ)
+  | notL u D => notL (γ u) (D.rename γ δ.cons)
+  | andR v D₁ D₂ => andR (δ v) (D₁.rename γ δ.cons) (D₂.rename γ δ.cons)
+  | andL₁ u D => andL₁ (γ u) (D.rename γ.cons δ)
+  | andL₂ u D => andL₂ (γ u) (D.rename γ.cons δ)
+  | orR₁ v D => orR₁ (δ v) (D.rename γ δ.cons)
+  | orR₂ v D => orR₂ (δ v) (D.rename γ δ.cons)
+  | orL u D₁ D₂ => orL (γ u) (D₁.rename γ.cons δ) (D₂.rename γ.cons δ)
+
+def Seq.id' (u : Mem A Γ) (v : Mem A Δ) : Seq Γ Δ :=
+  match A with
+  | .base _ => id u v
+  | .true => trueR v
+  | .false => falseL u
+  | .not _ => notR v (notL u.there (id' .here .here))
+  | .and .. => andR v (andL₁ u (id' .here .here)) (andL₂ u (id' .here .here))
+  | .or .. => orL u (orR₁ v (id' .here .here)) (orR₂ v (id' .here .here))
+
+@[simp]
+def Seq.sizeOf : (D : Seq Γ A) → Nat
+  | id .. | trueR _ | falseL _ => 0
+  | notR _ D | notL _ D | andL₁ _ D | andL₂ _ D | orR₁ _ D | orR₂ _ D => D.sizeOf + 1
+  | andR _ D₁ D₂ | orL _ D₁ D₂ => D₁.sizeOf + D₂.sizeOf + 1
+
+@[simp]
+theorem Seq.sizeOf_rename {γ : Rename Γ Γ'} {δ : Rename Δ Δ'} (D : Seq Γ Δ) : (D.rename γ δ).sizeOf = D.sizeOf :=
+  by induction D generalizing Γ' Δ' <;> simp! only [*]
+
+def Seq.cut : (D : Seq Γ (Δ.cons A)) → (E : Seq (Γ.cons A) Δ) → Seq Γ Δ
+  | .id u .here, E => E.rename (.contraction u) .id
+  | .id u (.there v), _ => .id u v
+  | D, .id .here v => D.rename .id (.contraction v)
+  | _, .id (.there u) v => .id u v
+  | D@(notR .here D₁), E@(notL .here E₁) => cut (cut (D.rename .id (.cons .weakening)) E₁) (cut D₁ (E.rename (.cons .weakening) .id))
+  | D@(andR .here D₁ _), E@(andL₁ .here E₁) => cut (cut (D₁.rename .id .exchange) (E.rename .id .weakening)) (cut (D.rename .weakening .id) (E₁.rename .exchange .id))
+  | D@(andR .here _ D₂), E@(andL₂ .here E₂) => cut (cut (D₂.rename .id .exchange) (E.rename .id .weakening)) (cut (D.rename .weakening .id) (E₂.rename .exchange .id))
+  | D@(orR₁ .here D₁), E@(orL .here E₁ _) => cut (cut (D₁.rename .id .exchange) (E.rename .id .weakening)) (cut (D.rename .weakening .id) (E₁.rename .exchange .id))
+  | D@(orR₂ .here D₂), E@(orL .here _ E₂) => cut (cut (D₂.rename .id .exchange) (E.rename .id .weakening)) (cut (D.rename .weakening .id) (E₂.rename .exchange .id))
+  | trueR (.there v), _ => trueR v
+  | falseL u, _ => falseL u
+  | notR (.there v) D, E => notR v (cut D (E.rename (.cons .weakening) .id))
+  | notL u D, E => notL u (cut (D.rename .id .exchange) (E.rename .id .weakening))
+  | andR (.there v) D₁ D₂, E => andR v (cut (D₁.rename .id .exchange) (E.rename .id .weakening)) (cut (D₂.rename .id .exchange) (E.rename .id .weakening))
+  | andL₁ u D, E => andL₁ u (cut D (E.rename (.cons .weakening) .id))
+  | andL₂ u D, E => andL₂ u (cut D (E.rename (.cons .weakening) .id))
+  | orR₁ (.there v) D, E => orR₁ v (cut (D.rename .id .exchange) (E.rename .id .weakening))
+  | orR₂ (.there v) D, E => orR₂ v (cut (D.rename .id .exchange) (E.rename .id .weakening))
+  | orL u D₁ D₂, E => orL u (cut D₁ (E.rename (.cons .weakening) .id)) (cut D₂ (E.rename (.cons .weakening) .id))
+  | _, trueR v => trueR v
+  | _, falseL (.there u) => falseL u
+  | D, notR v E => notR v (cut (D.rename .weakening .id) (E.rename .exchange .id))
+  | D, notL (.there u) E => notL u (cut (D.rename .id (.cons .weakening)) E)
+  | D, andR v E₁ E₂ => andR v (cut (D.rename .id (.cons .weakening)) E₁) (cut (D.rename .id (.cons .weakening)) E₂)
+  | D, andL₁ (.there u) E => andL₁ u (cut (D.rename .weakening .id) (E.rename .exchange .id))
+  | D, andL₂ (.there u) E => andL₂ u (cut (D.rename .weakening .id) (E.rename .exchange .id))
+  | D, orR₁ v E => orR₁ v (cut (D.rename .id (.cons .weakening)) E)
+  | D, orR₂ v E => orR₂ v (cut (D.rename .id (.cons .weakening)) E)
+  | D, orL (.there u) E₁ E₂ => orL u (cut (D.rename .weakening .id) (E₁.rename .exchange .id)) (cut (D.rename .weakening .id) (E₂.rename .exchange .id))
+  termination_by D E => (A, D.sizeOf, E.sizeOf)
+  decreasing_by all_goals subst_vars; decreasing_tactic
+
+end SC
